Add soundness proof for Cong decision procedure, WIP dead code decision procedure

src/Language/PlutusIR/Transform/Congruence.v
@@ -1,16 +1,28 @@
-Set Implicit Arguments.
-From PlutusCert Require Import Language.PlutusIR.
-From PlutusCert Require Import Language.PlutusIR.Analysis.Equality.
-From Equations Require Import Equations.
-Require Import Coq.Strings.String.
-Require Import Coq.Lists.List.
-From PlutusCert Require Import Util.List.
+From PlutusCert Require Import
+  Language.PlutusIR
+  Language.PlutusIR.Analysis.Equality
+  Util.List.
+
+From Equations Require Import
+  Equations.
+
+From Coq Require Import
+  Bool
+  Strings.String
+  Lists.List
+  Utf8
+  .
 
 Generalizable All Variables.
+Set Implicit Arguments.
 
 Section Congruence.
   Import NamedTerm.
-  Variables (R : Term -> Term -> Type) (S : list Binding -> list Binding -> Type).
+
+  Context
+    (R : Term -> Term -> Type)
+    (dec_R : Term -> Term -> bool)
+  .
 
   Inductive Cong_Binding : Binding -> Binding -> Type :=
     | C_TermBind     : `{ R t t' -> Cong_Binding (TermBind s v t)
@@ -50,33 +62,153 @@ Section Congruence.
                                                     (Unwrap t')}
   .
 
-    Definition is_cong_binding (is_R : Term -> Term -> bool) (b b' : Binding) : bool :=
+    Definition is_cong_binding  (b b' : Binding) : bool :=
       match b, b' with
-        | (TermBind s v t), (TermBind s' v' t') => Strictness_eqb s s' && VDecl_eqb v v' && is_R t t'
+        | (TermBind s v t), (TermBind s' v' t') => Strictness_eqb s s' && VDecl_eqb v v' && dec_R t t'
         | (TypeBind v T), (TypeBind v' T') => TVDecl_eqb v v'  && Ty_eqb T T'
         | (DatatypeBind d), (DatatypeBind d') => DTDecl_eqb d d'
         | _, _                               => false
       end
     .
 
-    Definition is_cong (is_R : Term -> Term -> bool) (t t' : Term) : bool :=
+    Definition is_cong (t t' : Term) : bool :=
       match t, t' with
-        | (Let r bs t), (Let r' bs' t')      => Recursivity_eqb r r' && forall2b (is_cong_binding is_R) bs bs' && is_R t t'
+        | (Let r bs t), (Let r' bs' t')      => Recursivity_eqb r r' && forall2b is_cong_binding bs bs' && dec_R t t'
         | (Var n), (Var n')                  => String.eqb n n'
-        | (TyAbs n k t), (TyAbs n' k' t')    => String.eqb n n' && Kind_eqb k k' && is_R t t'
-        | (LamAbs n T t), (LamAbs n' T' t')  => String.eqb n n'&& Ty_eqb T T' && is_R t t'
-        | (Apply s t), (Apply s' t')         => is_R s s' && is_R t t'
+        | (TyAbs n k t), (TyAbs n' k' t')    => String.eqb n n' && Kind_eqb k k' && dec_R t t'
+        | (LamAbs n T t), (LamAbs n' T' t')  => String.eqb n n'&& Ty_eqb T T' && dec_R t t'
+        | (Apply s t), (Apply s' t')         => dec_R s s' && dec_R t t'
         | (Constant v), (Constant v')        => some_valueOf_eqb v v'
         | (Builtin f), (Builtin f')          => func_eqb f f'
-        | (TyInst t T), (TyInst t' T')       => Ty_eqb T T' && is_R t t'
+        | (TyInst t T), (TyInst t' T')       => Ty_eqb T T' && dec_R t t'
         | (Error T), (Error T')              => Ty_eqb T T'
-        | (IWrap T1 T2 t), (IWrap T1' T2' t') => Ty_eqb T1 T1' && Ty_eqb T2 T2' && is_R t t'
-        | (Unwrap t), (Unwrap t')            => is_R t t'
+        | (IWrap T1 T2 t), (IWrap T1' T2' t') => Ty_eqb T1 T1' && Ty_eqb T2 T2' && dec_R t t'
+        | (Unwrap t), (Unwrap t')            => dec_R t t'
         | _, _                               => false
       end
       .
 
+    Ltac split_hypos :=
+      match goal with
+      | H : (?x && ?y)%bool = true |- _ => apply andb_true_iff in H; destruct H; split_hypos
+      | _ => idtac
+      end.
 
+    Axiom (String_eqb_eq       : ∀ x y, String.eqb x y = true -> x = y).
+    Axiom (Recursivity_eqb_eq  : ∀ x y, Recursivity_eqb x y = true -> x = y).
+    Axiom (Strictness_eqb_eq   : ∀ x y, Strictness_eqb x y = true -> x = y).
+    Axiom (Kind_eqb_eq         : ∀ x y, Kind_eqb x y = true -> x = y).
+    Axiom (Ty_eqb_eq           : ∀ x y, Ty_eqb x y = true -> x = y).
+    Axiom (some_valueOf_eqb_eq : ∀ x y, some_valueOf_eqb x y = true -> x = y).
+    Axiom (func_eqb_eq         : ∀ x y, func_eqb x y = true -> x = y).
+    Axiom (VDecl_eqb_eq        : ∀ x y, VDecl_eqb x y = true -> x = y).
+    Axiom (TVDecl_eqb_eq       : ∀ x y, TVDecl_eqb x y = true -> x = y).
+    Axiom (DTDecl_eqb_eq       : ∀ x y, DTDecl_eqb x y = true -> x = y).
+
+    Create HintDb Hints_soundness.
+    Hint Resolve
+      String_eqb_eq
+      Recursivity_eqb_eq
+      Strictness_eqb_eq
+      Kind_eqb_eq
+      Ty_eqb_eq
+      some_valueOf_eqb_eq
+      func_eqb_eq
+      VDecl_eqb_eq
+      TVDecl_eqb_eq
+      DTDecl_eqb_eq
+    : Hints_soundness.
+
+
+
+    Lemma is_cong_Binding_Cong_Binding : ∀ b b',
+        (∀ t t', dec_R t t' = true -> R t t') ->
+        is_cong_binding b b' = true -> Cong_Binding b b'.
+    Proof with eauto with Hints_soundness.
+      intros b b' H_term_sound H_dec.
+      destruct b, b'.
+      all: simpl in H_dec; try discriminate H_dec.
+      all: split_hypos.
+      - assert (s = s0)...
+        assert (v = v0)...
+        subst.
+        apply C_TermBind...
+      - assert (t = t1)...
+        assert (t0 = t2)...
+        subst.
+        apply C_TypeBind.
+      - assert (d = d0)...
+        subst.
+        apply C_DatatypeBind.
+    Qed.
+
+    Lemma is_cong_Bindings_Cong_Bindings : ∀ bs bs',
+        (∀ t t', dec_R t t' = true -> R t t') ->
+        forall2b is_cong_binding bs bs' = true -> Cong_Bindings bs bs'.
+    Proof with eauto.
+      intros bs.
+      induction bs.
+      all: intros bs' H_term_sound H_dec.
+      all: destruct bs'.
+      all: simpl in H_dec.
+      all: try discriminate H_dec.
+      - apply Cong_Bindings_Nil.
+      - split_hypos.
+        apply Cong_Bindings_Cons.
+        + apply is_cong_Binding_Cong_Binding...
+        + eauto.
+    Qed.
+
+    Lemma is_cong_Cong t t' :
+      (∀ t t', dec_R t t' = true -> R t t') ->
+      is_cong t t' = true -> Cong t t'.
+    Proof with eauto with Hints_soundness.
+      generalize t'.
+      clear t'.
+      intros t'.
+      induction t.
+      all: intros H_sound_R H_dec.
+      all: destruct t'.
+      all: simpl in H_dec.
+      all: try discriminate H_dec.
+      all: split_hypos.
+      - apply H_sound_R in H0.
+        apply Recursivity_eqb_eq in H.
+        subst.
+        eapply C_Let...
+        apply is_cong_Bindings_Cong_Bindings...
+      - apply String.eqb_eq in H_dec.
+        subst.
+        constructor.
+      - assert (b = s)...
+        assert (k = k0)...
+        subst.
+        eapply C_TyAbs...
+      - assert (b = s)...
+        assert (t = t1)...
+        subst.
+        apply C_LamAbs...
+      - apply C_Apply...
+      - assert (s = s0)...
+        subst.
+        apply C_Constant.
+      - assert (d = d0)... subst.
+        apply C_Builtin.
+      - assert (t0 = t1)... subst.
+        apply C_TyInst...
+      - assert (t = t0)... subst.
+        apply C_Error.
+      - assert (t = t2)...
+        assert (t0 = t3)...
+        subst.
+        apply C_IWrap...
+      - apply C_Unwrap...
+    Qed.
+
+
+
+
+    (* Constructors with explicit equalities for indices *)
     Definition C_TermBind'     : forall t t' s s' v v' , s = s' -> v = v' -> R t t' -> Cong_Binding
                                     (TermBind s  v t)
                                     (TermBind s' v' t').
@@ -96,70 +228,4 @@ Section Congruence.
   Notation "'Nothing'" := None.
   Notation "'Just'"    := Datatypes.Some.
 
-
-  Definition s2o a b : sumbool a b -> option a := fun x => match x with
-    | left x => Just x
-    | _      => Nothing
-    end.
-
-  Set Equations Transparent.
-
-  Variables r_dec : forall t1 t2, option (R t1 t2).
-  (*
-  Equations cong_dec : forall t1 t2, option (Cong t1 t2) :=
-    cong_dec (Let _ _ _) (Let _ _ _) := Nothing;
-
-    cong_dec (Var n)     (Var n')
-      with string_dec n n' =>
-     { | left eq_refl := Just C_Var;
-       | _            := Nothing  };
-
-    cong_dec (TyAbs n k t) (TyAbs n' k' t')
-      with (string_dec n n', Kind_dec k k', r_dec t t') =>
-     { | (left eq_refl, left eq_refl, Just r) := Just (C_TyAbs r);
-       | _  := Nothing};
-
-    cong_dec (LamAbs n ty t) (LamAbs n' ty' t')
-      with (string_dec n n', Ty_dec ty ty', r_dec t t') =>
-     { | (left eq_refl, left eq_refl, Just r) := Just (C_LamAbs r);
-       | _  := Nothing};
-
-    cong_dec (Apply t1 t2) (Apply t1' t2')
-      with (r_dec t1 t1', r_dec t2 t2') =>
-     { | (Just r, Just r') := Just (C_Apply r r');
-       | _  := Nothing};
-
-    cong_dec (Constant v) (Constant v')
-      with some_valueOf_dec v v' =>
-     { | left eq_refl := Just C_Constant;
-       | _       := Nothing};
-
-    cong_dec (Builtin f) (Builtin f')
-      with func_dec f f' =>
-    { | left eq_refl := Just C_Builtin;
-      | _ := Nothing
-    };
-
-    cong_dec (TyInst t ty) (TyInst t' ty')
-      with (r_dec t t', Ty_dec ty ty') =>
-     { | (Just r, left eq_refl) := Just (C_TyInst r);
-       | _  := Nothing};
-
-    cong_dec (Error ty) (Error ty')
-      with (Ty_dec ty ty') =>
-     { | (left eq_refl) := Just C_Error;
-       | _  := Nothing};
-
-    cong_dec (IWrap ty1 ty2 t) (IWrap ty1' ty2' t')
-      with (r_dec t t', Ty_dec ty1 ty1', Ty_dec ty2 ty2') =>
-     { | (Just r, left eq_refl, left eq_refl) := Just (C_IWrap r);
-       | _  := Nothing};
-
-    cong_dec (Unwrap t) (Unwrap t')
-      with (r_dec t t') =>
-     { | Just r := Just (C_Unwrap r);
-       | _  := Nothing};
-
-    cong_dec _           _           := Nothing.
-   *)
 End Congruence.
