src/Language/PlutusIR/Transform/DeadCode/DecideBool.v
@@ -1,0 +1,219 @@
+From Coq Require Import
+  String
+  List
+  Bool
+  Program
+  Utf8_core
+.
+
+From PlutusCert Require Import
+  Util
+  UniqueBinders
+  Purity
+  Language.PlutusIR
+  Language.PlutusIR.Analysis.Equality
+  Language.PlutusIR.Transform.Congruence
+  DeadBindings
+  Congruence
+.
+Import Congruence.
+
+Import NamedTerm.
+Import ListNotations.
+
+
+Section Bindings.
+
+  Context (dec_Term : Term -> Term -> bool).
+  Context (dec_Term_sound : ∀ s t, dec_Term s t = true -> dead_syn s t).
+
+  Set Diffs "on".
+
+
+  Fixpoint dec_Binding (b b' : Binding) : bool := match b, b' with
+    | TermBind s vd t, TermBind s' vd' t' => Strictness_eqb s s' && VDecl_eqb vd vd' && dec_Term t t'
+    | b, b' => Binding_eqb b b'
+    end.
+
+  Axiom (String_eqb_eq       : ∀ x y, String.eqb x y = true -> x = y).
+  Axiom (Recursivity_eqb_eq  : ∀ x y, Recursivity_eqb x y = true -> x = y).
+  Axiom (Strictness_eqb_eq   : ∀ x y, Strictness_eqb x y = true -> x = y).
+  Axiom (Kind_eqb_eq         : ∀ x y, Kind_eqb x y = true -> x = y).
+  Axiom (Ty_eqb_eq           : ∀ x y, Ty_eqb x y = true -> x = y).
+  Axiom (some_valueOf_eqb_eq : ∀ x y, some_valueOf_eqb x y = true -> x = y).
+  Axiom (func_eqb_eq         : ∀ x y, func_eqb x y = true -> x = y).
+  Axiom (VDecl_eqb_eq        : ∀ x y, VDecl_eqb x y = true -> x = y).
+  Axiom (TVDecl_eqb_eq       : ∀ x y, TVDecl_eqb x y = true -> x = y).
+  Axiom (DTDecl_eqb_eq       : ∀ x y, DTDecl_eqb x y = true -> x = y).
+
+  Create HintDb Hints_soundness.
+  Hint Resolve
+    String_eqb_eq
+    Recursivity_eqb_eq
+    Strictness_eqb_eq
+    Kind_eqb_eq
+    Ty_eqb_eq
+    some_valueOf_eqb_eq
+    func_eqb_eq
+    VDecl_eqb_eq
+    TVDecl_eqb_eq
+    DTDecl_eqb_eq
+  : Hints_soundness.
+
+  Hint Constructors
+    and
+  : Hints_soundness.
+
+
+  Axiom dec_Binding_sound : ∀ b b', dec_Binding b b' = true -> dead_syn_binding b b'.
+
+  Hint Resolve
+    dec_Binding_sound
+  : Hints_soundness.
+
+  Definition safely_removed b bsn :=
+    negb (existsb (String.eqb (name_Binding b)) bsn) &&
+    is_pure_binding [] b.
+
+  Definition binding_was_there b' bs : bool :=
+    match find (λ b, String.eqb (name_Binding b) (name_Binding b')) bs with
+      | Datatypes.Some b => dec_Binding b b'
+      | None => false
+    end
+    .
+
+  (* inlined and specialized `find` for termination checking *)
+  Definition find_Binding b' :=
+  fix find (bs : list Binding) : bool :=
+    match bs with
+    | []      => false
+    | b :: bs => if String.eqb (name_Binding b) (name_Binding b') then dec_Binding b b' else find bs
+    end.
+
+  (* This does not work in the termination checker, it doesn't see that b returned by find 
+     is a structural subterm.
+     It would have to fuse the result of find (an option string) with the resulting, which is
+     what I did in the above definition*)
+  Definition find_Binding' b' bs :=
+    match find (λ b, String.eqb (name_Binding b) (name_Binding b')) bs with
+      | Datatypes.Some b => dec_Binding b b'
+      | None => false
+    end.
+
+
+  Definition dec_Bindings (bs bs' : list Binding) : bool :=
+    let bsn := map name_Binding bs in
+    let bs'n := map name_Binding bs' in
+    forallb (fun b => safely_removed b bs'n) bs &&
+    forallb (fun b' =>
+    find_Binding b' bs
+    ) bs'.
+
+  (* this did not pass termination checking *)
+  (*
+    forallb (fun b' =>
+    match find (λ b, String.eqb (name_Binding b) (name_Binding b')) bs with
+      | Datatypes.Some b => dec_Binding b b'
+      | None => false
+    end
+    ) bs'
+   *)
+
+  Lemma H_safely_removed bs bs':
+      forallb (fun b => safely_removed b (map name_Binding bs')) bs = true ->
+      ∀ b : Binding, In b bs → name_removed b bs' → pure_binding [] b.
+  Proof with eauto with Hints_soundness.
+    intros H_dec.
+    intros b H_In H_removed.
+    unfold safely_removed in H_dec.
+    rewrite forallb_forall in H_dec. (* why did rewrite accept a <-> ? was also possible with eapply -> ..., but generated an existential for x *)
+    apply H_dec in H_In as H_dec_andb.
+    clear H_dec H_In.
+    apply andb_true_iff in H_dec_andb.
+    destruct H_dec_andb as [_ H_dec_pure_binding].
+    apply is_pure_binding_pure_binding.
+    assumption.
+  Qed.
+
+  Lemma H_find_binding bs bs' :
+      forallb (fun b' => find_Binding b' bs) bs' = true ->
+      ∀ b', In b' bs' ->
+         ∃ x, In x bs /\
+           name_Binding x = name_Binding b' /\
+           dead_syn_binding x b'
+      .
+  Proof with eauto with Hints_soundness.
+    rewrite forallb_forall.
+    intros H_dec b' H_In.
+    apply H_dec in H_In.
+    clear H_dec.
+    induction bs as [ | b ].
+    - discriminate H_In.
+    - simpl in H_In.
+      destruct (String.eqb (name_Binding b) (name_Binding b')) eqn:H_name_eq.
+
+      (* b related to b' *)
+      + exists b.
+        repeat split...
+        * constructor...
+
+      (* a not related to b' *)
+      + apply IHbs in H_In. clear IHbs.
+        destruct H_In as [x [H_x_In [H_eq_name H_dead_syn]]].
+        assert (In x (b :: bs)). { apply in_cons... }
+        exists x...
+  Qed.
+
+  Create HintDb Hints_bindings.
+  Hint Resolve
+    H_safely_removed
+    H_find_binding.
+  Hint Constructors
+    dead_syn_bindings.
+
+  Ltac split_hypos :=
+    match goal with
+    | H : (?x && ?y)%bool = true |- _ => apply andb_true_iff in H; destruct H; split_hypos
+    | _ => idtac
+    end.
+
+  Lemma dec_Bindings_sound : ∀ bs bs',
+    dec_Bindings bs bs' = true -> dead_syn_bindings bs bs'.
+  Proof with eauto with Hints_bindings.
+    intros bs bs' H.
+    simpl in H.
+    unfold dec_Bindings in H.
+    split_hypos.
+    eapply dc_bindings...
+  Qed.
+
+
+End Bindings.
+
+Fixpoint dec_Term (x y : Term) {struct x} : bool := match x, y with
+
+  | Let r bs t   , Let r' bs' t' => if dec_Bindings dec_Term bs bs'
+        then Recursivity_eqb r r' && dec_Term t t'
+        else forallb (is_pure_binding []) bs && dec_Term t t' (* Check whether the whole let was removed *)
+
+  | _, _ => is_cong dec_Term x y
+
+  end
+.
+
+Lemma dec_Term_sound t t' :
+  dec_Term t t' = true -> dead_syn t t'.
+Proof.
+  intros H_dec.
+  induction t.
+  2: {
+    unfold dec_Term in H_dec.
+    simpl in H_dec.
+  
+
+From Coq Require Import Extraction.
+Extraction Language Haskell.
+Recursive Extraction dec_Term.
+Require Import Strings.Ascii.
+Recursive Extraction nat_of_ascii.
+Recursive Extraction ascii_of_nat.
